aarch64 ainvs: prove cur_vcpu_in_cur_domain
Show that if there is a current VCPU then the TCB bound to it is always
in the current domain.

While this property should also hold for ARM_HYP, it is currently only
proven for AARCH64. This is because the property is defined with
projections that do not yet exist for ARM_HYP.

Signed-off-by: Corey Lewis <corey.lewis@proofcraft.systems>

proof/invariant-abstract/AARCH64/ArchVCPU_AI.thy
@@ -186,7 +186,7 @@ lemma tcb_cur_fpu_update_active_cur_vcpu_of[wp]:
 
 crunch lazy_fpu_restore
   for active_cur_vcpu_of[wp]: "\<lambda>s. P (active_cur_vcpu_of s)"
-  and tcb_vcpu_at[wp]: "arch_tcb_at (\<lambda>itcb. P (itcb_vcpu itcb)) t"
+  and arch_tcb_vcpu_at[wp]: "arch_tcb_at (\<lambda>itcb. P (itcb_vcpu itcb)) t"
   (ignore: arch_thread_set wp: crunch_wps)
 
 crunch set_vm_root, set_tcb_queue, lazy_fpu_restore
@@ -876,6 +876,569 @@ lemma call_kernel_valid_cur_vcpu:
   apply (simp flip: bind_assoc)
   by (wpsimp wp: handle_event_valid_cur_vcpu hoare_vcg_if_lift2 hoare_drop_imps
       | strengthen invs_valid_idle)+
+
+
+section \<open>cur_vcpu_in_cur_domain\<close>
+
+\<comment> \<open> Show that the TCB bound to the current VCPU is in the current domain. \<close>
+
+\<comment> \<open>FIXME: @{term cur_vcpu} could be reworked so that it could be reused here\<close>
+definition cur_vcpu_tcb :: "'z::state_ext state \<Rightarrow> obj_ref option" where
+  "cur_vcpu_tcb s \<equiv>
+     case arm_current_vcpu (arch_state s) of
+       Some (v, _) \<Rightarrow> vcpu_tcbs_of s v
+     | None \<Rightarrow> None"
+
+definition cur_vcpu_in_cur_domain :: "det_ext state \<Rightarrow> bool" where
+  "cur_vcpu_in_cur_domain s \<equiv>
+     case cur_vcpu_tcb s of
+       Some t \<Rightarrow> in_cur_domain t s
+     | None \<Rightarrow> True"
+
+lemmas cur_vcpu_in_cur_domain_defs = cur_vcpu_in_cur_domain_def cur_vcpu_tcb_def in_cur_domain_def
+
+lemma cur_vcpu_in_cur_domain_lift_strong:
+  assumes [wp]: "\<And>P. f \<lbrace>\<lambda>s. P (arm_current_vcpu (arch_state s))\<rbrace>"
+                "\<And>P. f \<lbrace>\<lambda>s. P (vcpu_tcbs_of s)\<rbrace>"
+                "\<And>P. f \<lbrace>\<lambda>s. P (cur_domain s)\<rbrace>"
+                "\<And>P t. f \<lbrace>etcb_at (\<lambda>t. P (etcb_domain t)) t\<rbrace>"
+  shows "f \<lbrace>cur_vcpu_in_cur_domain\<rbrace>"
+  unfolding cur_vcpu_in_cur_domain_defs
+  by (wp_pre, wps, wpsimp wp: valid_case_option_post_wp split: option.splits)
+
+lemma cur_vcpu_in_cur_domain_lift:
+  assumes "\<And>P. f \<lbrace>\<lambda>s. P (arm_current_vcpu (arch_state s))\<rbrace>"
+          "\<And>P. f \<lbrace>\<lambda>s. P (vcpu_tcbs_of s)\<rbrace>"
+          "\<And>P. f \<lbrace>\<lambda>s. P (cur_domain s)\<rbrace>"
+          "\<And>P. f \<lbrace>\<lambda>s. P (etcbs_of s)\<rbrace>"
+  shows "f \<lbrace>cur_vcpu_in_cur_domain\<rbrace>"
+ by (rule cur_vcpu_in_cur_domain_lift_strong assms)+
+
+\<comment> \<open>This simp could possibly be avoided if arm_current_vcpu updates were wrapped in a function
+    instead of directly using modifies.\<close>
+lemma cur_vcpu_in_cur_domain_current_vcpu_update[simp]:
+  "cur_vcpu_in_cur_domain (s\<lparr>arch_state := arch_state s\<lparr>arm_current_vcpu := Some (v, b)\<rparr>\<rparr>)
+   = (\<forall>t. vcpu_tcbs_of s v = Some t \<longrightarrow> in_cur_domain t s)"
+  "cur_vcpu_in_cur_domain (s\<lparr>arch_state := arch_state s\<lparr>arm_current_vcpu := None\<rparr>\<rparr>)"
+  by (auto simp: cur_vcpu_in_cur_domain_defs split: option.splits)
+
+\<comment> \<open>FIXME: use projections instead of this\<close>
+lemma cur_vcpu_in_cur_domain_updates[simp]:
+  "cur_vcpu_in_cur_domain (cur_thread_update f_ct s) = cur_vcpu_in_cur_domain s"
+  "cur_vcpu_in_cur_domain (machine_state_update f_ms s) = cur_vcpu_in_cur_domain s"
+  "cur_vcpu_in_cur_domain (cdt_update f_cdt s) = cur_vcpu_in_cur_domain s"
+  "cur_vcpu_in_cur_domain (cdt_list_update f_cdt_list s) = cur_vcpu_in_cur_domain s"
+  "cur_vcpu_in_cur_domain (work_units_completed_update f_work_units s) = cur_vcpu_in_cur_domain s"
+  "cur_vcpu_in_cur_domain (interrupt_states_update f_interrupt_states s) = cur_vcpu_in_cur_domain s"
+  "cur_vcpu_in_cur_domain (is_original_cap_update f_orig_cap s) = cur_vcpu_in_cur_domain s"
+  "cur_vcpu_in_cur_domain (arch_state_update (arm_asid_table_update f_asid_table) s) = cur_vcpu_in_cur_domain s"
+  "cur_vcpu_in_cur_domain (s\<lparr>arch_state := (arm_asid_table_update f_asid_table) (arch_state s)\<rparr>) = cur_vcpu_in_cur_domain s"
+  by (auto simp: cur_vcpu_in_cur_domain_defs)
+
+\<comment> \<open>schedule\<close>
+
+lemma as_user_vcpus_of[wp]:
+  "as_user t f \<lbrace>\<lambda>s. P (vcpus_of s)\<rbrace>"
+  unfolding as_user_def
+  by (wpsimp wp: set_object_wp_strong)
+     (fastforce simp: opt_map_def obj_at_def split: option.splits elim!: rsubst[where P=P])
+
+crunch set_scheduler_action, tcb_sched_action, as_user
+  for cur_vcpu_in_cur_domain[wp]: cur_vcpu_in_cur_domain
+  (wp: cur_vcpu_in_cur_domain_lift)
+
+lemma vcpu_write_reg_vcpu_tcbs_of[wp]:
+  "vcpu_write_reg vr reg val \<lbrace>\<lambda>s. P (vcpu_tcbs_of s)\<rbrace>"
+  unfolding vcpu_write_reg_def
+  by wpsimp (fastforce simp: opt_map_def elim!: rsubst[where P=P])
+
+lemma vgic_update_vcpu_tcbs_of[wp]:
+  "vgic_update vr f \<lbrace>\<lambda>s. P (vcpu_tcbs_of s)\<rbrace>"
+  unfolding vgic_update_def
+  by wpsimp (fastforce simp: opt_map_def elim!: rsubst[where P=P])
+
+lemma vcpu_save_reg_vcpu_tcbs_of[wp]:
+  "vcpu_save_reg vr reg \<lbrace>\<lambda>s. P (vcpu_tcbs_of s)\<rbrace>"
+  unfolding vcpu_save_reg_def
+  apply wpsimp
+  by (fastforce simp: opt_map_def elim!: rsubst[where P=P])
+
+lemma save_virt_timer_vcpu_tcbs_of[wp]:
+  "save_virt_timer vcpu_ptr \<lbrace>\<lambda>s. P (vcpu_tcbs_of s)\<rbrace>"
+  unfolding save_virt_timer_def
+  apply wpsimp
+         apply (rule hoare_post_imp[where Q'="\<lambda>_ s. P (vcpu_tcbs_of s)"])
+          apply (fastforce simp: opt_map_def elim!: rsubst[where P=P])
+         by wpsimp+
+
+crunch vcpu_disable, vcpu_restore, vcpu_save
+  for vcpu_tcbs_of[wp]: "\<lambda>s. P (vcpu_tcbs_of s)"
+  (wp: crunch_wps)
+
+lemma vcpu_switch_cur_vcpu_in_cur_domain[wp]:
+  "\<lbrace>\<lambda>s. cur_vcpu_in_cur_domain s \<and> none_top ((\<lambda>t. in_cur_domain t s) |< vcpu_tcbs_of s) v\<rbrace>
+   vcpu_switch v
+   \<lbrace>\<lambda>_. cur_vcpu_in_cur_domain\<rbrace>"
+  unfolding vcpu_switch_def
+  apply (wpsimp wp: hoare_vcg_all_lift hoare_vcg_imp_lift in_cur_domain_lift_weak)
+  by (auto simp: cur_vcpu_in_cur_domain_defs opt_pred_def)
+
+crunch set_vm_root, lazy_fpu_restore
+  for vcpus_of[wp]: "\<lambda>s. P (vcpus_of s)"
+  and arm_current_vcpu[wp]: "\<lambda>s. P (arm_current_vcpu (arch_state s))"
+  (wp: crunch_wps set_object_wp_strong simp: crunch_simps)
+
+crunch set_vm_root, set_global_user_vspace, lazy_fpu_restore
+  for cur_vcpu_in_cur_domain[wp]: cur_vcpu_in_cur_domain
+  (wp: cur_vcpu_in_cur_domain_lift)
+
+lemma arch_switch_to_thread_cur_vcpu_in_cur_domain[wp]:
+  "\<lbrace>\<lambda>s. cur_vcpu_in_cur_domain s \<and> valid_objs s \<and> in_cur_domain t s \<and> sym_refs (state_hyp_refs_of s)\<rbrace>
+   arch_switch_to_thread t
+   \<lbrace>\<lambda>_. cur_vcpu_in_cur_domain\<rbrace>"
+  unfolding arch_switch_to_thread_def
+  apply wpsimp
+  apply (frule (1) valid_tcb_objs)
+  apply (clarsimp simp: valid_tcb_def valid_arch_tcb_def typ_at_eq_kheap_obj)
+  apply (drule (1) bound_tcb_bound_vcpu_at[where tcbptr=t])
+   apply (fastforce simp: pred_tcb_def2)
+  apply (auto simp: in_omonad)
+  done
+
+crunch guarded_switch_to, switch_to_idle_thread
+  for cur_vcpu_in_cur_domain[wp]: cur_vcpu_in_cur_domain
+  (wp: crunch_wps)
+
+lemma choose_thread_cur_vcpu_in_cur_domain[wp]:
+  "\<lbrace>\<lambda>s. cur_vcpu_in_cur_domain s \<and> valid_queues s \<and> valid_objs s \<and> sym_refs (state_hyp_refs_of s)\<rbrace>
+   choose_thread
+   \<lbrace>\<lambda>_. cur_vcpu_in_cur_domain\<rbrace>"
+  unfolding choose_thread_def
+  apply wpsimp
+  apply (fastforce dest!: next_thread_queued split: option.splits
+                   simp: etcb_at_def next_thread_def valid_queues_def in_cur_domain_def)
+  done
+
+lemma next_domain_cur_vcpu_in_cur_domain[wp]:
+  "\<lbrace>\<lambda>s. arm_current_vcpu (arch_state s) = None\<rbrace> next_domain \<lbrace>\<lambda>_. cur_vcpu_in_cur_domain\<rbrace>"
+  unfolding next_domain_def Let_def
+  by (wpsimp wp: dxo_wp_weak simp: cur_vcpu_in_cur_domain_defs)
+
+lemma vcpu_flush_arm_current_vcpu_None[wp]:
+  "\<lbrace>\<top>\<rbrace> vcpu_flush \<lbrace>\<lambda>_ s. arm_current_vcpu (arch_state s) = None\<rbrace>"
+  unfolding vcpu_flush_def
+  by wpsimp
+
+crunch next_domain, vcpu_flush, switch_local_fpu_owner
+  for hyp_refs_of[wp]: "\<lambda>s. P (state_hyp_refs_of s)"
+  and valid_objs[wp]: valid_objs
+  (simp: crunch_simps wp: dxo_wp_weak crunch_wps ignore: arch_thread_set)
+
+lemma schedule_choose_new_thread_cur_vcpu_in_cur_domain[wp]:
+  "\<lbrace>\<lambda>s. cur_vcpu_in_cur_domain s \<and> valid_queues s \<and> valid_objs s \<and> sym_refs (state_hyp_refs_of s)\<rbrace>
+   schedule_choose_new_thread
+   \<lbrace>\<lambda>_. cur_vcpu_in_cur_domain\<rbrace>"
+  unfolding schedule_choose_new_thread_def arch_prepare_next_domain_def
+  by wpsimp
+
+lemma schedule_cur_vcpu_in_cur_domain[wp]:
+  "\<lbrace>\<lambda>s. cur_vcpu_in_cur_domain s \<and> valid_sched s \<and> valid_objs s \<and> sym_refs (state_hyp_refs_of s)\<rbrace>
+   schedule
+   \<lbrace>\<lambda>_. cur_vcpu_in_cur_domain\<rbrace>"
+  unfolding schedule_def schedule_switch_thread_fastfail_def
+  apply (wpsimp wp: hoare_drop_imps gts_wp)
+  by (safe; (fastforce simp: valid_sched_def valid_sched_action_def weak_valid_sched_action_def
+                             switch_in_cur_domain_def st_tcb_at_def obj_at_def)?)
+
+
+\<comment> \<open>handle_interrupt\<close>
+
+lemma set_endpoint_vcpus_of[wp]:
+  "set_endpoint p ep \<lbrace>\<lambda>s. P (vcpus_of s)\<rbrace>"
+  unfolding set_simple_ko_def
+  by (wpsimp wp: set_object_wp get_object_wp)
+     (fastforce simp: opt_map_def obj_at_def elim!: rsubst[where P=P])
+
+lemma set_notification_vcpus_of[wp]:
+  "set_notification p ntfn \<lbrace>\<lambda>s. P (vcpus_of s)\<rbrace>"
+  unfolding set_simple_ko_def
+  by (wpsimp wp: set_object_wp get_object_wp)
+     (fastforce simp: opt_map_def obj_at_def elim!: rsubst[where P=P])
+
+lemma thread_set_vcpus_of[wp]:
+  "thread_set p t \<lbrace>\<lambda>s. P (vcpus_of s)\<rbrace>"
+  unfolding thread_set_def
+  by (wpsimp wp: set_object_wp)
+     (fastforce simp: opt_map_def get_tcb_def split: option.splits elim!: rsubst[where P=P])
+
+lemma set_bound_notification_vcpus_of[wp]:
+  "set_bound_notification p ntfn \<lbrace>\<lambda>s. P (vcpus_of s)\<rbrace>"
+  unfolding set_bound_notification_def
+  by (wpsimp wp: set_object_wp)
+     (fastforce simp: opt_map_def get_tcb_def split: option.splits elim!: rsubst[where P=P])
+
+crunch store_word_offs
+  for vcpus_of[wp]: "\<lambda>s. P (vcpus_of s)"
+
+lemma set_mrs_vcpus_of[wp]:
+  "set_mrs thread buf msgs \<lbrace>\<lambda>s. P (vcpus_of s)\<rbrace>"
+  unfolding set_mrs_def zipWithM_x_mapM
+  by (wpsimp wp: mapM_wp[where S=UNIV] set_object_wp)
+     (fastforce simp: opt_map_def get_tcb_def split: option.splits elim!: rsubst[where P=P])
+
+crunch set_extra_badge, handle_fault
+  for vcpus_of[wp]: "\<lambda>s. P (vcpus_of s)"
+  (wp: crunch_wps transfer_caps_loop_pres
+   simp: crunch_simps
+   ignore: set_simple_ko)
+
+lemma vppi_event_vcpu_tcbs_of[wp]:
+  "vppi_event irq \<lbrace>\<lambda>s. P (vcpu_tcbs_of s)\<rbrace>"
+  unfolding vppi_event_def
+  by (wpsimp)
+     (fastforce simp: opt_map_def get_tcb_def split: option.splits elim!: rsubst[where P=P])
+
+crunch handle_interrupt
+  for vcpu_tcbs_of[wp]: "\<lambda>s. P (vcpu_tcbs_of s)"
+  and cur_vcpu_in_cur_domain[wp]: cur_vcpu_in_cur_domain
+  (wp: cur_vcpu_in_cur_domain_lift_strong dxo_wp_weak crunch_wps
+   simp: crunch_simps
+   ignore: set_simple_ko)
+
+
+\<comment> \<open>handle_event\<close>
+
+lemma retype_region_cur_vcpu_in_cur_domain[wp]:
+  "retype_region ptr numObjects o_bits type dev \<lbrace>cur_vcpu_in_cur_domain\<rbrace>"
+  unfolding retype_region_def
+  apply (wpsimp simp_del: fun_upd_apply simp: foldr_fun_upd_value)
+  by (auto simp: cur_vcpu_in_cur_domain_defs etcb_at'_def
+                 default_object_def default_arch_object_def default_tcb_def default_arch_tcb_def
+                 default_vcpu_def opt_map_def etcbs_of'_def
+          split: option.splits apiobject_type.splits aobject_type.splits)
+
+crunch do_machine_op, create_cap, init_arch_objects
+  for cur_vcpu_in_cur_domain[wp]: cur_vcpu_in_cur_domain
+  (wp: cur_vcpu_in_cur_domain_lift crunch_wps simp: crunch_simps)
+
+lemma delete_objects_cur_vcpu_in_cur_domain[wp]:
+  "delete_objects ptr bits \<lbrace>cur_vcpu_in_cur_domain\<rbrace>"
+  unfolding delete_objects_def
+  apply wpsimp
+   apply (rule hoare_strengthen_post, rule do_machine_op_cur_vcpu_in_cur_domain)
+  by (auto simp: cur_vcpu_in_cur_domain_defs etcb_at'_def detype_def opt_map_def etcbs_of'_def
+          split: option.splits)
+
+crunch invoke_untyped
+  for cur_vcpu_in_cur_domain[wp]: cur_vcpu_in_cur_domain
+  (wp: crunch_wps mapME_x_wp' preemption_point_inv' simp: crunch_simps mapM_x_def_bak) \<comment> \<open>FIXME: change invoke_untyped to use mapM_x\<close>
+
+lemma set_vcpu_None_cur_vcpu_in_cur_domain[wp]:
+  "set_vcpu vcpu_ptr (v\<lparr>vcpu_tcb := None\<rparr>) \<lbrace>cur_vcpu_in_cur_domain\<rbrace>"
+  unfolding cur_vcpu_in_cur_domain_defs
+  apply (wp_pre, wps, wpsimp)
+  by (auto split: option.splits simp: opt_map_def)
+
+crunch arch_thread_set, vcpu_disable
+  for cur_vcpu_in_cur_domain[wp]: cur_vcpu_in_cur_domain
+  (wp: cur_vcpu_in_cur_domain_lift crunch_wps simp: crunch_simps)
+
+lemma vcpu_invalidate_active_cur_vcpu_in_cur_domain[wp]:
+  "\<lbrace>\<top>\<rbrace> vcpu_invalidate_active \<lbrace>\<lambda>_. cur_vcpu_in_cur_domain\<rbrace>"
+  unfolding vcpu_invalidate_active_def
+  by wpsimp
+
+lemma dissociate_vcpu_tcb_cur_vcpu_in_cur_domain[wp]:
+  "dissociate_vcpu_tcb vcpu_ptr tcb_ptr \<lbrace>cur_vcpu_in_cur_domain\<rbrace>"
+  unfolding dissociate_vcpu_tcb_def
+  by (wpsimp wp: hoare_drop_imps)
+
+crunch cap_move, suspend, delete_asid_pool, unmap_page, cancel_badged_sends
+  for etcb_at[wp]: "etcb_at P t"
+  and cur_domain[wp]: "\<lambda>s. P (cur_domain s)"
+  (wp: crunch_wps dxo_wp_weak simp: crunch_simps filterM_mapM)
+
+crunch
+  cap_insert, cap_move, cap_swap, set_thread_state, unbind_maybe_notification, unbind_notification,
+  cancel_all_ipc, suspend, cancel_all_signals, delete_asid_pool, unmap_page, delete_asid,
+  unmap_page_table, cancel_badged_sends, empty_slot, fpu_release
+  for vcpu_tcbs_of[wp]: "\<lambda>s. P (vcpu_tcbs_of s)"
+  and arm_current_vcpu[wp]: "\<lambda>s. P (arm_current_vcpu (arch_state s))"
+  and cur_vcpu_in_cur_domain[wp]: cur_vcpu_in_cur_domain
+  (wp: cur_vcpu_in_cur_domain_lift_strong crunch_wps dxo_wp_weak
+   simp: crunch_simps filterM_mapM
+   ignore: set_simple_ko tcb_sched_action)
+
+crunch invoke_cnode
+  for cur_vcpu_in_cur_domain[wp]: cur_vcpu_in_cur_domain
+  (wp: crunch_wps preemption_point_inv' cap_revoke_preservation dxo_wp_weak
+   simp: crunch_simps)
+
+crunch set_priority
+  for etcb_at_domain[wp]: "etcb_at (\<lambda>t. P (etcb_domain t)) t"
+  and cur_domain[wp]: "\<lambda>s. P (cur_domain s)"
+  (wp: thread_set_no_change_etcb_at)
+
+crunch set_mcpriority, bind_notification
+  for etcb_at[wp]: "etcb_at P t"
+  and cur_domain[wp]: "\<lambda>s. P (cur_domain s)"
+  (wp: crunch_wps thread_set_no_change_etcb_at simp: crunch_simps etcb_of_def)
+
+crunch cancel_ipc, set_mcpriority, set_priority, bind_notification
+  for vcpu_tcbs_of[wp]: "\<lambda>s. P (vcpu_tcbs_of s)"
+  and arm_current_vcpu[wp]: "\<lambda>s. P (arm_current_vcpu (arch_state s))"
+  and cur_vcpu_in_cur_domain[wp]: cur_vcpu_in_cur_domain
+  (wp: cur_vcpu_in_cur_domain_lift_strong ignore: set_simple_ko)
+
+lemma thread_set_no_etcb_change_cur_vcpu_in_cur_domain:
+  assumes x: "\<And>P tcb. P (tcb_domain (f tcb)) = (P (tcb_domain tcb) :: bool)"
+  shows      "thread_set f t' \<lbrace>cur_vcpu_in_cur_domain\<rbrace>"
+  by (wpsimp wp: cur_vcpu_in_cur_domain_lift_strong thread_set_no_change_etcb_at simp: x)
+
+lemma option_update_thread_no_etcb_change_cur_vcpu_in_cur_domain:
+  assumes x: "\<And>P val tcb. P (tcb_domain (f val tcb)) = (P (tcb_domain tcb) :: bool)"
+  shows      "option_update_thread t f opt \<lbrace>cur_vcpu_in_cur_domain\<rbrace>"
+  unfolding option_update_thread_def
+  by (wpsimp wp: cur_vcpu_in_cur_domain_lift_strong thread_set_no_change_etcb_at simp: x)
+
+crunch invoke_tcb
+  for cur_vcpu_in_cur_domain[wp]: cur_vcpu_in_cur_domain
+  (wp: crunch_wps check_cap_inv thread_set_no_etcb_change_cur_vcpu_in_cur_domain
+       option_update_thread_no_etcb_change_cur_vcpu_in_cur_domain)
+
+lemma set_vcpu_not_current_cur_vcpu_in_cur_domain:
+  "\<lbrace>\<lambda>s. cur_vcpu_in_cur_domain s \<and> map_option fst (arm_current_vcpu (arch_state s)) \<noteq> Some vcpu_ptr\<rbrace>
+   set_vcpu vcpu_ptr v
+   \<lbrace>\<lambda>_. cur_vcpu_in_cur_domain\<rbrace>"
+  unfolding cur_vcpu_in_cur_domain_defs
+  apply (wp_pre, wps, wpsimp)
+  by (auto split: option.splits simp: opt_map_def)
+
+lemma dissociate_vcpu_tcb_not_current_vcpu[wp]:
+  "\<lbrace>\<top>\<rbrace> dissociate_vcpu_tcb vcpu_ptr tcb_ptr \<lbrace>\<lambda>_ s. map_option fst (arm_current_vcpu (arch_state s)) \<noteq> Some vcpu_ptr\<rbrace>"
+  unfolding dissociate_vcpu_tcb_def
+  by (wpsimp wp: get_vcpu_wp arch_thread_get_wp vcpu_invalid_active_arm_current_vcpu_None[THEN hoare_strengthen_post])
+
+crunch dissociate_vcpu_tcb
+  for vcpus_of_None[wp]: "\<lambda>s. vcpus_of s vcpu_ptr = None"
+  (wp: hoare_vcg_imp_lift' get_vcpu_wp arch_thread_get_wp simp: if_option_eq)
+
+crunch dissociate_vcpu_tcb
+  for scheduler_action[wp]: "\<lambda>s. P (scheduler_action s)"
+  (wp: crunch_wps)
+
+lemma vcpu_invalidate_active_cur_vcpu[wp]:
+  "\<lbrace>\<top>\<rbrace> vcpu_invalidate_active \<lbrace>\<lambda>_ s. cur_vcpu_2 (arm_current_vcpu (arch_state s)) (P s)\<rbrace>"
+  unfolding vcpu_invalidate_active_def cur_vcpu_def
+  by wpsimp
+
+lemma dissociate_vcpu_tcb_cur_vcpu[wp]:
+  "dissociate_vcpu_tcb vcpu_ptr tcb_ptr \<lbrace>cur_vcpu\<rbrace>"
+  unfolding dissociate_vcpu_tcb_def
+  apply (wpsimp wp: hoare_vcg_imp_lift' get_vcpu_wp arch_thread_get_wp | wps)+
+  apply (clarsimp simp: cur_vcpu_def in_omonad split: option.splits)
+  done
+
+lemma associate_vcpu_tcb_cur_vcpu_in_cur_domain[wp]:
+  "\<lbrace>cur_vcpu_in_cur_domain and ct_in_cur_domain and cur_vcpu and (\<lambda>s. tcb_ptr \<noteq> idle_thread s)
+    and (\<lambda>s. scheduler_action s = resume_cur_thread)\<rbrace>
+   associate_vcpu_tcb vcpu_ptr tcb_ptr
+   \<lbrace>\<lambda>_. cur_vcpu_in_cur_domain\<rbrace>" (is "\<lbrace>?P\<rbrace> _ \<lbrace>_\<rbrace>")
+  unfolding associate_vcpu_tcb_def
+  apply wpsimp
+        apply (solves \<open>(wpsimp wp: hoare_vcg_imp_lift' set_vcpu_not_current_cur_vcpu_in_cur_domain get_vcpu_wp
+                        | wps
+                        | clarsimp simp: in_omonad)+\<close>)+
+    apply (rule_tac Q'="\<lambda>_. ?P" in hoare_post_imp)
+     apply (fastforce simp: in_omonad ct_in_cur_domain_def cur_vcpu_def)
+    apply (wpsimp | wps)+
+  done
+
+lemma invoke_vcpu_ack_vppi_vcpu_tcbs_of[wp]:
+  "invoke_vcpu_ack_vppi vcpu_ptr vppi \<lbrace>\<lambda>s. P (vcpu_tcbs_of s)\<rbrace>"
+  unfolding invoke_vcpu_ack_vppi_def
+  apply wpsimp
+  by (fastforce simp: opt_map_def elim!: rsubst[where P=P])
+
+crunch invoke_vcpu_inject_irq, invoke_vcpu_write_register, invoke_vcpu_ack_vppi
+  for vcpu_tcbs_of[wp]: "\<lambda>s. P (vcpu_tcbs_of s)"
+  and arm_current_vcpu[wp]: "\<lambda>s. P (arm_current_vcpu (arch_state s))"
+  and cur_vcpu_in_cur_domain[wp]: cur_vcpu_in_cur_domain
+  (wp: cur_vcpu_in_cur_domain_lift_strong)
+
+crunch invoke_vcpu_read_register
+  for cur_vcpu_in_cur_domain[wp]: cur_vcpu_in_cur_domain
+
+lemma perform_vcpu_invocation_cur_vcpu_in_cur_domain[wp]:
+  "\<lbrace>cur_vcpu_in_cur_domain and ct_in_cur_domain and cur_vcpu and valid_vcpu_invocation vi
+    and (\<lambda>s. scheduler_action s = resume_cur_thread)\<rbrace>
+   perform_vcpu_invocation vi
+   \<lbrace>\<lambda>_. cur_vcpu_in_cur_domain\<rbrace>"
+  unfolding perform_vcpu_invocation_def
+  by (wpsimp simp: valid_vcpu_invocation_def)
+
+crunch store_pte, store_asid_pool_entry
+  for cur_vcpu_in_cur_domain[wp]: cur_vcpu_in_cur_domain
+  (wp: cur_vcpu_in_cur_domain_lift)
+
+crunch
+  perform_vspace_invocation, perform_page_table_invocation, perform_page_invocation,
+  perform_asid_control_invocation, perform_asid_pool_invocation, perform_sgi_invocation
+  for cur_vcpu_in_cur_domain[wp]: cur_vcpu_in_cur_domain
+  (wp: crunch_wps  simp: crunch_simps)
+
+lemma arch_perform_invocation_cur_vcpu_in_cur_domain[wp]:
+  "\<lbrace>cur_vcpu_in_cur_domain and ct_in_cur_domain and cur_vcpu and valid_arch_inv ai
+    and (\<lambda>s. scheduler_action s = resume_cur_thread)\<rbrace>
+   arch_perform_invocation ai
+   \<lbrace>\<lambda>_. cur_vcpu_in_cur_domain\<rbrace>"
+  unfolding arch_perform_invocation_def
+  by (wpsimp simp: valid_arch_inv_def)
+
+lemma thread_set_domain_cur_vcpu_in_cur_domain[wp]:
+  "\<lbrace>\<lambda>s. cur_vcpu_in_cur_domain s \<and> sym_refs (state_hyp_refs_of s) \<and> valid_objs s
+        \<and> (arm_current_vcpu (arch_state s) = None
+           \<or> arch_tcb_at (\<lambda>itcb. itcb_vcpu itcb \<noteq> map_option fst (arm_current_vcpu (arch_state s))) tptr s
+           \<or> cur_domain s = new_dom)\<rbrace>
+   thread_set_domain tptr new_dom
+   \<lbrace>\<lambda>_. cur_vcpu_in_cur_domain\<rbrace>"
+  unfolding thread_set_domain_def thread_set_def
+  apply (wpsimp wp: set_object_wp)
+  by (auto simp: cur_vcpu_in_cur_domain_defs pred_tcb_at_def obj_at_def etcb_at_def etcbs_of'_def
+          split: option.splits dest: bound_vcpu_bound_tcb_at)
+
+lemma set_domain_cur_vcpu_in_cur_domain[wp]:
+  "\<lbrace>\<lambda>s. cur_vcpu_in_cur_domain s \<and> sym_refs (state_hyp_refs_of s) \<and> valid_objs s
+        \<and> (arm_current_vcpu (arch_state s) = None
+           \<or> arch_tcb_at (\<lambda>itcb. itcb_vcpu itcb \<noteq> map_option fst (arm_current_vcpu (arch_state s))) tptr s
+           \<or> cur_domain s = new_dom)\<rbrace>
+   set_domain tptr new_dom
+   \<lbrace>\<lambda>_. cur_vcpu_in_cur_domain\<rbrace>"
+  unfolding set_domain_def
+  by (wpsimp wp: thread_set_domain_cur_vcpu_in_cur_domain hoare_vcg_disj_lift | wps)+
+
+crunch fpu_release
+  for arch_tcb_vcpu_at[wp]: "\<lambda>s. (arch_tcb_at (\<lambda>itcb. P (itcb_vcpu itcb)) t s)"
+  (simp: crunch_simps wp: crunch_wps)
+
+lemma vcpu_flush_if_current_make_vcpu_safe[wp]:
+  "\<lbrace>\<top>\<rbrace>
+   vcpu_flush_if_current tptr
+   \<lbrace>\<lambda>_ s. arm_current_vcpu (arch_state s) = None
+          \<or> arch_tcb_at (\<lambda>itcb. itcb_vcpu itcb \<noteq> map_option fst (arm_current_vcpu (arch_state s))) tptr s\<rbrace>"
+  unfolding vcpu_flush_if_current_def
+  apply (wpsimp wp: vcpu_flush_arm_current_vcpu_None[THEN hoare_strengthen_post] arch_thread_get_wp)
+  apply (clarsimp simp: pred_tcb_at_def obj_at_def)
+  done
+
+lemma arch_prepare_set_domain_make_vcpu_safe[wp]:
+  "\<lbrace>\<top>\<rbrace>
+   arch_prepare_set_domain tptr new_dom
+   \<lbrace>\<lambda>_ s. arm_current_vcpu (arch_state s) = None
+          \<or> arch_tcb_at (\<lambda>itcb. itcb_vcpu itcb \<noteq> map_option fst (arm_current_vcpu (arch_state s))) tptr s
+          \<or> cur_domain s = new_dom\<rbrace>"
+  unfolding arch_prepare_set_domain_def
+  by (wpsimp wp: hoare_vcg_disj_lift[where f="fpu_release tptr"]
+                 vcpu_flush_if_current_make_vcpu_safe[THEN hoare_strengthen_post]
+      | wps)+
+
+lemma vcpu_flush_cur_vcpu_in_cur_domain[wp]:
+  "\<lbrace>\<top>\<rbrace> vcpu_flush \<lbrace>\<lambda>_. cur_vcpu_in_cur_domain\<rbrace>"
+  unfolding vcpu_flush_def
+  by (wpsimp simp: cur_vcpu_in_cur_domain_defs)
+
+crunch arch_prepare_set_domain
+  for hyp_refs_of[wp]: "\<lambda>s. P (state_hyp_refs_of s)"
+  and valid_objs[wp]: valid_objs
+  and cur_vcpu_in_cur_domain[wp]: cur_vcpu_in_cur_domain
+  (wp: crunch_wps simp: crunch_simps)
+
+lemma invoke_domain_cur_vcpu_in_cur_domain[wp]:
+  "\<lbrace>\<lambda>s. cur_vcpu_in_cur_domain s \<and> sym_refs (state_hyp_refs_of s) \<and> valid_objs s\<rbrace>
+   invoke_domain thread domain
+   \<lbrace>\<lambda>_. cur_vcpu_in_cur_domain\<rbrace>"
+  unfolding invoke_domain_def
+  by wpsimp
+
+crunch do_reply_transfer, handle_recv, handle_vm_fault
+  for etcb_at[wp]: "etcb_at P t"
+  and cur_domain[wp]: "\<lambda>s. P (cur_domain s)"
+  (wp: crunch_wps preemption_point_inv' simp: crunch_simps filterM_mapM)
+
+crunch do_reply_transfer, handle_recv, handle_vm_fault
+  for vcpu_tcbs_of[wp]: "\<lambda>s. P (vcpu_tcbs_of s)"
+  and arm_current_vcpu[wp]: "\<lambda>s. P (arm_current_vcpu (arch_state s))"
+  and cur_vcpu_in_cur_domain[wp]: cur_vcpu_in_cur_domain
+  (wp: cur_vcpu_in_cur_domain_lift_strong crunch_wps dxo_wp_weak
+   simp: crunch_simps
+   ignore: set_simple_ko)
+
+crunch
+  handle_fault, reply_from_kernel, send_ipc, send_signal, invoke_irq_control, invoke_irq_handler,
+  reschedule_required, handle_hypervisor_fault
+  for cur_vcpu_in_cur_domain[wp]: cur_vcpu_in_cur_domain
+  (wp: cur_vcpu_in_cur_domain_lift_strong dxo_wp_weak crunch_wps
+   simp: crunch_simps)
+
+lemma perform_invocation_cur_vcpu_in_cur_domain[wp]:
+  "\<lbrace>cur_vcpu_in_cur_domain and ct_in_cur_domain and cur_vcpu and valid_invocation iv
+    and valid_objs and (\<lambda>s. sym_refs (state_hyp_refs_of s))
+    and (\<lambda>s. scheduler_action s = resume_cur_thread)\<rbrace>
+   perform_invocation blocking call iv
+   \<lbrace>\<lambda>_. cur_vcpu_in_cur_domain\<rbrace>"
+  by (case_tac iv, simp_all; (solves wpsimp)?)
+
+lemma set_thread_state_runnable_scheduler_action:
+  "\<lbrace>\<lambda>s. P (scheduler_action s) \<and> runnable ts\<rbrace> set_thread_state t ts \<lbrace>\<lambda>_ s. P (scheduler_action s)\<rbrace>"
+  apply (simp add: set_thread_state_def)
+  apply (simp add: set_thread_state_act_def set_object_def get_object_def set_scheduler_action_def)
+  apply (wpsimp wp: gts_wp)
+  by (clarsimp simp: pred_tcb_at_def obj_at_def)
+
+lemma handle_invocation_cur_vcpu_in_cur_domain[wp]:
+  "\<lbrace>cur_vcpu_in_cur_domain and invs and ct_in_cur_domain and ct_active
+    and (\<lambda>s. scheduler_action s = resume_cur_thread)\<rbrace>
+   handle_invocation calling blocking
+   \<lbrace>\<lambda>_. cur_vcpu_in_cur_domain\<rbrace>"
+  unfolding handle_invocation_def
+  apply (wpsimp wp: syscall_valid)
+          apply (wp gts_wp hoare_vcg_all_lift hoare_drop_imps cur_vcpu_typ_lift
+                    set_thread_state_runnable_scheduler_action
+                | simp add: split_def)+
+  apply (fastforce simp: invs_def valid_state_def valid_arch_state_def valid_pspace_def
+                         valid_tcb_state_def ct_in_state_def
+                  elim!: pred_tcb_weakenE)
+  done
+
+crunch maybe_handle_interrupt
+  for cur_vcpu_in_cur_domain[wp]: cur_vcpu_in_cur_domain
+
+lemma handle_event_cur_vcpu_in_cur_domain[wp]:
+  "\<lbrace>cur_vcpu_in_cur_domain and invs and ct_in_cur_domain and (\<lambda>s. e \<noteq> Interrupt \<longrightarrow> ct_active s)
+    and (\<lambda>s. scheduler_action s = resume_cur_thread)\<rbrace>
+   handle_event e
+   \<lbrace>\<lambda>_. cur_vcpu_in_cur_domain\<rbrace>"
+  apply (cases e; clarsimp; (solves wpsimp)?)
+  unfolding handle_call_def handle_send_def handle_reply_def handle_yield_def
+  by (wpsimp wp: get_cap_wp)+
+
+crunch activate_thread
+  for cur_vcpu_in_cur_domain[wp]: cur_vcpu_in_cur_domain
+
+lemma call_kernel_cur_vcpu_in_cur_domain:
+  "\<lbrace>cur_vcpu_in_cur_domain and invs and valid_sched and (\<lambda>s. e \<noteq> Interrupt \<longrightarrow> ct_active s)
+    and (\<lambda>s. scheduler_action s = resume_cur_thread)\<rbrace>
+   call_kernel e
+   \<lbrace>\<lambda>_. cur_vcpu_in_cur_domain\<rbrace>"
+  unfolding call_kernel_def maybe_handle_interrupt_def
+  apply (wpsimp wp: handle_spurious_irq_invs| strengthen invs_valid_objs invs_hyp_sym_refs)+
+    (* simplify postcondition by ruling out non_kernel_IRQs *)
+    apply (rule hoare_post_imp[where Q'="\<lambda>irq s. irq \<notin> Some ` non_kernel_IRQs \<and> cur_vcpu_in_cur_domain s \<and> valid_sched s \<and> invs s"])
+     apply fastforce
+    apply (wpsimp wp: getActiveIRQ_neq_non_kernel handle_event_valid_sched
+           | strengthen invs_valid_objs invs_hyp_sym_refs)+
+  apply (clarsimp simp: valid_sched_def)
+  done
 
 end
 
